spc/Hoareproof2.v
@@ -34,12 +34,12 @@ Section CANCEL.
 
 
 
+  Context `{SK: Sk.ld}.
   Context `{Σ: GRA.t}.
-  Context `{X: Sk.ld}.
 
   Variable mds: list SMod.t.
 
-  Let sk: Sk.sem := Sk.canon (fold_right Sk.add Sk.unit (List.map SMod.sk mds)).
+  Let sk: Sk.t := Sk.canon (fold_right Sk.add Sk.unit (List.map SMod.sk mds)).
   (* Let skenv: SkEnv.t := Sk.load_skenv sk. *)
   Let mss: list SModSem.t := (List.map ((flip SMod.get_modsem) sk) mds).
   Let sbtb: list (gname * fspecbody) := (List.flat_map (SModSem.fnsems) mss).
@@ -96,7 +96,7 @@ Section CANCEL.
     Beh.of_program (ModL.compile (Mod.add_list mds_src)).
   Proof.
     eapply ModSem.refines_close.
-    eapply (@adequacy_local_list_strong X mds_src mds_mid2).
+    eapply (@adequacy_local_list_strong _ mds_src mds_mid2).
     unfold mds_src, mds_mid2.
     eapply Forall2_apply_Forall2.
     { refl. }
